proof/DDC/Language/SimplePCFa/ExpLift.v
@@ -4,10 +4,7 @@ Require Import DDC.Language.SimplePCFa.Exp.
 (* Lifting of references into the environment *)
 Fixpoint liftXV (d: nat) (vv: val) : val := 
   match vv with
-  | VVar i
-  => if le_gt_dec d i
-       then VVar (S i)
-       else vv
+  | VVar i       => if le_gt_dec d i then VVar (S i) else vv
   | VConst c     => VConst c
   | VLam t x     => VLam t (liftXX (S d) x)
   | VFix t v     => VFix t (liftXV (S d) v)
@@ -15,11 +12,11 @@ Fixpoint liftXV (d: nat) (vv: val) : val :=
 
 with    liftXX (d: nat) (xx: exp) : exp :=
   match xx with
-  | XVal v       => XVal (liftXV d v)
+  | XVal v       => XVal   (liftXV d v)
   | XLet t x1 x2 => XLet t (liftXX d x1) (liftXX (S d) x2)
   | XApp v1 v2   => XApp   (liftXV d v1) (liftXV d v2)
   | XOp1 o v     => XOp1 o (liftXV d v)
-  | XIf v1 x2 x3 => XIf  (liftXV d v1) (liftXX d x2) (liftXX d x3)
+  | XIf v1 x2 x3 => XIf    (liftXV d v1) (liftXX d x2) (liftXX d x3)
   end.
 
 
