proof/DDC/Language/SimplePCFa/ExpLower.v
@@ -1,0 +1,40 @@
+
+Require Import DDC.Language.SimplePCFa.Exp.
+Require Import DDC.Language.SimplePCFa.ExpLift.
+
+
+(* Lifting of references into the environment *)
+Fixpoint lowerXV (d: nat) (vv: val) : val := 
+  match vv with
+  | VVar    O    => vv
+  | VVar (S i)   => if le_gt_dec d (S i) then VVar i else vv
+  | VConst c     => VConst c
+  | VLam t x     => VLam t (lowerXX (S d) x)
+  | VFix t v     => VFix t (lowerXV (S d) v)
+  end
+
+with    lowerXX (d: nat) (xx: exp) : exp :=
+  match xx with
+  | XVal v       => XVal   (lowerXV d v)
+  | XLet t x1 x2 => XLet t (lowerXX d x1) (lowerXX (S d) x2)
+  | XApp v1 v2   => XApp   (lowerXV d v1) (lowerXV d v2)
+  | XOp1 o v     => XOp1 o (lowerXV d v)
+  | XIf v1 x2 x3 => XIf    (lowerXV d v1) (lowerXX d x2) (lowerXX d x3)
+  end.
+
+
+Lemma lowerXX_liftXX_id
+ : forall d x
+ , lowerXX d (liftXX d x) = x.
+Proof.
+ intros. gen d.
+ induction x using exp_mutind with
+  (PV := fun v => forall d, lowerXV d (liftXV d v) = v); 
+  intros; simpl; try burn.
+
+  SCase "VVar".
+    repeat (simpl; lift_cases; try burn).
+   destruct n;
+    repeat (simpl; lift_cases; try burn).
+Qed.
+    
